More work on maps

Maps.v
@@ -1,6 +1,5 @@
 Require Export externals.QuantumLib.Prelim.
 Require Import Coq.Arith.Peano_dec.
-Require Import stdpp.fin_maps.
 
 Definition partial_map A : Type := (list nat) * (nat -> option A).
 
@@ -67,6 +66,9 @@ Definition contains {A} (pm : partial_map A) (key : nat) :=
   (keys, _) => Inb key keys 
   end.
 
+Definition get {A} (pm : partial_map A) (key : nat) :=
+  if (contains pm key) then (snd pm) key else None.
+
 Definition size {A} (pm : partial_map A) := 
   match pm with
   (keys, _) => length keys
@@ -75,13 +77,13 @@ Definition size {A} (pm : partial_map A) :=
 Fixpoint to_list_helper {A} (keys : list nat) (map : nat -> option A) : list (nat * A) :=
   match keys with
   | [] => []
-  | key :: keys' => match (map key) with
+  | key :: keys' => match get (keys, map) key with
                     | None => to_list_helper keys' map
                     | Some v => (key, v) :: to_list_helper keys' map
                     end
   end.
 
-Notation "a !! pm" := ((snd pm) a) (at level 20).
+Notation "a !! pm" := (get pm a) (at level 20).
 Notation "a ?? pm" := (contains pm a) (at level 20).
 Notation "<[ key ↦ val ; pm ]>" := (insert pm key val) (at level 30).
 Notation "<[ key ↦ val ]>" := (insert empty_map key val) (at level 30).
@@ -106,8 +108,10 @@ Lemma insert_Some : forall {A} (pm : partial_map A) key (a : A),
   key !! (<[ key ↦ a; pm ]>) = Some a.
 Proof.
   intros.
-  unfold insert.
+  unfold get.
   destruct pm.
+  rewrite insert_contains.
+  unfold insert.
   simpl.
   rewrite Nat.eqb_refl.
   easy.
@@ -144,17 +148,6 @@ Proof.
         easy.
 Qed.
 
-Lemma remove_None : forall {A} (pm : partial_map A) key , 
-  key !! (<[ pm -- key]>) = None.
-Proof.
-  intros.
-  unfold remove.
-  destruct pm.
-  simpl.
-  rewrite Nat.eqb_refl.
-  easy.
-Qed.
-
 Lemma remove_no_contains : forall {A} (pm : partial_map A) key,
   key ?? (<[ pm -- key]>) = false.
 Proof.
@@ -165,6 +158,17 @@ Proof.
   rewrite Not_Inb_In.
   apply remove_In.
 Qed.
+
+Lemma remove_None : forall {A} (pm : partial_map A) key , 
+  key !! (<[ pm -- key]>) = None.
+Proof.
+  intros.
+  destruct pm.
+  unfold get.
+  rewrite remove_no_contains.
+  easy.
+Qed.
+
 
 Lemma remove_contains_size : forall {A} (pm : partial_map A) key,
   key ?? pm = true -> (size (<[ pm -- key]>)) < size pm.
@@ -179,89 +183,204 @@ Proof.
   assumption.
 Qed.
 
-Definition graph_multi_map := partial_map (partial_map nat).
-
-Definition multi_add (gmm : graph_multi_map) from to :=
-  match (from !! gmm) with
-  | None => <[ from ↦ (<[to ↦ 1]>); gmm ]>
-  | Some m => match (to !! m) with
-              | None => <[ from ↦ (<[to ↦ 1; m]>); gmm ]>
-              | Some n' => <[ from ↦ (<[to ↦ S n'; m]>); gmm ]>
-              end
-  end.
-
-Definition multi_remove (gmm : graph_multi_map) from to :=
-  match (from !! gmm) with
-  | None => gmm
-  | Some m => match (to !! m) with
-              | None => gmm
-              | Some n' => <[ from ↦ (<[to ↦ (pred n'); m]>); gmm ]>
-              end
-  end.
-
-Definition multi_clear (gmm : graph_multi_map) from to :=
-    match (from !! gmm) with
-    | None => gmm
-    | Some m => match (to !! m) with
-                | None => gmm
-                | Some n' => <[ from ↦ (<[m -- to]>); gmm ]>
-                end
-    end.
-
-Definition multi_get (gmm : graph_multi_map) from to :=
-  match (from !! gmm) with
-  | None => 0
-  | Some m => match (to !! m) with
-              | None => 0
-              | Some v => v
-              end
-  end.
-
-Notation "( from , to ) !!! gmm" := (multi_get gmm from to) (at level 20).
-Notation "( from , to ) ++ gmm" := (multi_add gmm from to) (at level 20).
-Notation "( from , to ) -- gmm" := (multi_remove gmm from to) (at level 20).
-Notation "( from , to ) ~~ gmm" := (multi_clear gmm from to) (at level 20).
-
-Lemma multi_add_increases : forall (gmm : graph_multi_map) from to,
-  S ((from, to) !!! gmm) = (from, to) !!! ((from,to) ++ gmm).
+Lemma get_implies_contains : forall {A} (pm : partial_map A) key a, key !! pm = Some a -> key ?? pm = true.
 Proof.
   intros.
-  unfold multi_get, multi_add.
-  destruct (from !! gmm).
-  - destruct (to !! p); rewrite 2 insert_Some; easy.
-  - rewrite 2 insert_Some; easy.
+  unfold get in H.
+  destruct (key ?? pm); [ reflexivity | discriminate H ].
 Qed.
 
-Lemma multi_remove_decreases : forall (gmm : graph_multi_map) from to,
-  pred ((from, to) !!! gmm) = (from, to) !!! ((from,to) -- gmm).
+
+Lemma empty_no_contains : forall {A} (pm : partial_map A) key, size pm = 0 -> key ?? pm = false.
 Proof.
   intros.
-  unfold multi_get, multi_remove.
-  destruct (from !! gmm) eqn:H.
-  - destruct (to !! p) eqn:H1.
-    + rewrite 2 insert_Some.
-      easy.
-    + rewrite H.
-      rewrite H1.
-      reflexivity. 
-  - rewrite H. easy.
+  destruct pm.
+  unfold size in H.
+  rewrite length_zero_iff_nil in H.
+  simpl.
+  subst.
+  easy.
 Qed.
 
-Lemma multi_clear_0 : forall (gmm : graph_multi_map) from to,
-  0 = (from, to) !!! ((from,to) ~~ gmm).
+Lemma In_if_lookup : forall {A} (pm : partial_map A) key a, (forall x y : A, {x = y} + {x <> y}) -> key !! pm = Some a -> In (key, a) (to_list pm).
 Proof.
   intros.
-  unfold multi_get, multi_clear.
-  destruct (from !! gmm) eqn:H.
-  - destruct (to !! p) eqn:H1.
-    + rewrite insert_Some.
-      rewrite remove_None.
-      easy.
-    + rewrite H.
-      rewrite H1.
-      reflexivity. 
-  - rewrite H. easy.
+  generalize dependent a.
+  generalize dependent key.
+  destruct pm.
+  induction l; intros.
+  - simpl.
+    simpl in H.
+    discriminate.
+  - simpl.
+    destruct (o a) eqn:H'.
+    + simpl.
+      specialize (X a1 a0).
+      destruct X.
+      * subst.
+        bdestruct (a =? key).
+        subst.
+        rewrite H.
+        -- left.
+           easy.
+        -- unfold get.
+           simpl.
+           rewrite Nat.eqb_refl.
+           rewrite H'.
+           right.
+           apply IHl.
+           simpl in H.
+           unfold get in *.
+           simpl in H.
+           bdestruct (a =? key); [ contradiction | ].
+           destruct (Inb key l) eqn: H2.
+           ++ simpl.
+              rewrite H2.
+              apply H.
+           ++ discriminate H.   
+      * simpl in IHl.
+        bdestruct (key =? a).
+        -- subst.
+           rewrite H.
+           right.
+           unfold get in H.
+           simpl in H.
+           rewrite Nat.eqb_refl in H.
+           destruct (a ?? (l, o)) eqn:H1.
+           ++ apply IHl.
+              unfold get.
+              rewrite H1.
+              simpl.
+              assumption.
+           ++ exfalso.
+              rewrite H in H'.
+              inversion H'.
+              contradict n.
+              symmetry.
+              apply H2.
+        -- simpl.
+           unfold get.
+           simpl.
+           rewrite Nat.eqb_refl.
+           rewrite H'.
+           right.
+           apply IHl.
+           unfold get in H.
+           simpl in H.
+           bdestruct (a =? key); [ symmetry in H1; contradiction | ].
+           unfold get.
+           simpl.
+           assumption.
+    + simpl in IHl.
+      unfold get.
+      simpl.
+      rewrite Nat.eqb_refl.
+      rewrite H'.
+      apply IHl.
+      unfold get in H.
+      simpl in H.
+      bdestruct (a =? key).
+      * exfalso.
+        subst.
+        rewrite H in H'.
+        discriminate H'.
+      * unfold get.
+        simpl.
+        apply H.
 Qed.
+
+Lemma Lookup_if_in : forall {A} (pm : partial_map A) key a, (forall x y : A, {x = y} + {x <> y}) -> In (key, a) (to_list pm) -> key !! pm = Some a.
+Proof.
+  intros.
+  generalize dependent key.
+  generalize dependent a.
+  destruct pm.
+  induction l; intros.
+  - simpl in H.
+    contradiction.
+  - simpl in H.
+    unfold get.
+    simpl.
+    bdestruct (a =? key).
+    + unfold get in H.
+      simpl in H.
+      rewrite Nat.eqb_refl in H.
+      destruct (o a) eqn:H'.
+      * simpl in H.
+        specialize (X a0 a1).
+        simpl in IHl.
+        destruct H.
+        rewrite pair_equal_spec in H.
+        destruct H.
+        subst.
+        assumption.
+        specialize (IHl a0 key).
+        unfold get in IHl.
+        destruct (key ?? (l, o)) eqn:H''.
+        ++ simpl in IHl.
+           apply IHl.
+           assumption.
+        ++ specialize (IHl H).
+           discriminate IHl.  
+      * subst.
+        specialize (IHl a0 key).
+        unfold get in IHl.
+        destruct (key ?? (l, o)) eqn:H''.
+        ++ simpl in IHl.
+           apply IHl.
+           assumption.
+        ++ simpl in IHl.
+           specialize (IHl H).
+           discriminate.
+    + unfold get in H.
+      simpl in H.
+      rewrite Nat.eqb_refl in H.
+      simpl.
+      specialize (IHl a0 key).
+      unfold get in IHl.
+      simpl in IHl.
+      apply IHl.
+      destruct (o a) eqn:H'.
+      * simpl in H.
+        destruct H.
+        ++ apply pair_equal_spec in H.
+           destruct H.
+           subst.
+           contradiction.
+        ++ exact H.
+      * exact H.   
+Qed.
+
+Lemma contain_to_list : forall {A} (pm : partial_map A) key a,
+  (forall x y : A, {x = y} + {x <> y}) -> key ?? pm = true -> key !! pm = Some a -> In (key, a) (to_list pm).
+Proof.
+  intros.
+  destruct pm.
+  generalize dependent a.
+  induction l; intros.
+  - simpl in H.
+    discriminate H.
+  - simpl.
+    simpl in IHl.
+    destruct (o a).
+    + simpl.
+      simpl in H0.
+      simpl in H.
+      bdestruct (a =? key).
+      * simpl.
+        left.
+        admit.
+      * right.
+        apply IHl; assumption.
+    + apply IHl.
+      simpl in H.
+      simpl in H0.
+      bdestruct (a =? key).
+      * admit. 
+      * assumption.
+      * simpl in H0.
+        assumption.
+Qed. 
 
 Definition map {A B} (pm : partial_map A) (f : A -> B) : partial_map B :=
   match pm with
@@ -302,10 +421,176 @@ Definition map_opt {A B} (pm : partial_map A) (f : A -> option B) : partial_map 
                     )
 end.
 
-Definition get_keys {A} (pm : partial_map A) : list nat :=
-  match pm with
-  (keys, map) => keys
+Definition graph_multi_map := partial_map (partial_map nat).
+
+Definition multi_add (gmm : graph_multi_map) from to :=
+  match (from !! gmm) with
+  | None => <[ from ↦ (<[to ↦ 1]>); gmm ]>
+  | Some m => match (to !! m) with
+              | None => <[ from ↦ (<[to ↦ 1; m]>); gmm ]>
+              | Some n' => <[ from ↦ (<[to ↦ S n'; m]>); gmm ]>
+              end
   end.
+
+Definition multi_remove (gmm : graph_multi_map) from to :=
+  match (from !! gmm) with
+  | None => gmm
+  | Some m => match (to !! m) with
+              | None => gmm
+              | Some n' => <[ from ↦ (<[to ↦ (pred n'); m]>); gmm ]>
+              end
+  end.
+
+Definition multi_clear (gmm : graph_multi_map) from to :=
+    match (from !! gmm) with
+    | None => gmm
+    | Some m => match (to !! m) with
+                | None => gmm
+                | Some n' => <[ from ↦ (<[m -- to]>); gmm ]>
+                end
+    end.
+
+Definition multi_get (gmm : graph_multi_map) from to :=
+  match (from !! gmm) with
+  | None => 0
+  | Some m => match (to !! m) with
+              | None => 0
+              | Some v => v
+              end
+  end.
+
+Notation "<( from , to )> !!! gmm" := (multi_get gmm from to) (at level 20).
+Notation "<( from , to )> ++ gmm" := (multi_add gmm from to) (at level 20).
+Notation "<( from , to )> -- gmm" := (multi_remove gmm from to) (at level 20).
+Notation "<( from , to )> ~~ gmm" := (multi_clear gmm from to) (at level 20).
+
+
+Definition is_adjancent (gmm: graph_multi_map) from to :=
+  <(from,to)> !!! gmm > 0.
+
+
+Lemma multi_add_increases : forall (gmm : graph_multi_map) from to,
+  S (<(from, to)> !!! gmm) = <(from, to)> !!! (<(from,to)> ++ gmm).
+Proof.
+  intros.
+  unfold multi_get, multi_add.
+  destruct (from !! gmm).
+  - destruct (to !! p); rewrite 2 insert_Some; easy.
+  - rewrite 2 insert_Some; easy.
+Qed.
+
+Lemma multi_add_adjacent : forall (gmm : graph_multi_map) from to,
+  is_adjancent (<(from,to)> ++ gmm) from to.
+Proof.
+  intros.
+  unfold is_adjancent.
+  rewrite <- multi_add_increases.
+  apply gt_Sn_O.
+Qed.
+
+Lemma multi_remove_decreases : forall (gmm : graph_multi_map) from to,
+  pred (<(from, to)> !!! gmm) = <(from, to)> !!! (<(from,to)> -- gmm).
+Proof.
+  intros.
+  unfold multi_get, multi_remove.
+  destruct (from !! gmm) eqn:H.
+  - destruct (to !! p) eqn:H1.
+    + rewrite 2 insert_Some.
+      easy.
+    + rewrite H.
+      rewrite H1.
+      reflexivity. 
+  - rewrite H. easy.
+Qed.
+
+Lemma multi_remove_not_adjacent_1 : forall (gmm : graph_multi_map) from to,
+  (<(from, to)> !!! gmm) <= 1 -> ~ is_adjancent (<(from,to)> -- gmm) from to.
+Proof.
+  intros.
+  unfold is_adjancent.
+  rewrite <- multi_remove_decreases.
+  destruct (<(from, to)> !!! gmm); [ | destruct (<(from, to)> !!! gmm)].
+  1,2: simpl;unfold not; intros; inversion H0.
+  all: inversion H; subst; simpl.
+  - contradict H3.
+    auto.
+  - inversion H3.
+  - inversion H.
+    subst.
+    discriminate H4.
+  - inversion H4.
+  - inversion H.
+    simpl.
+    unfold not; intros.
+    inversion H0.
+    inversion H1.
+  - inversion H1. 
+Qed.
+
+Lemma multi_remove_adjacent_gt_1 : forall (gmm : graph_multi_map) from to,
+  (<(from, to)> !!! gmm) > 1 -> is_adjancent (<(from,to)> -- gmm) from to.
+Proof.
+  intros.
+  unfold is_adjancent.
+  rewrite <- multi_remove_decreases.
+  destruct (<(from, to)> !!! gmm).
+  - inversion H.
+  - rewrite pred_Sn.
+    simpl.
+    apply gt_S_n.
+    assumption.
+Qed.
+
+Lemma multi_clear_0 : forall (gmm : graph_multi_map) from to,
+  0 = <(from, to)> !!! (<(from,to)> ~~ gmm).
+Proof.
+  intros.
+  unfold multi_get, multi_clear.
+  destruct (from !! gmm) eqn:H.
+  - destruct (to !! p) eqn:H1.
+    + rewrite insert_Some.
+      rewrite remove_None.
+      easy.
+    + rewrite H.
+      rewrite H1.
+      reflexivity. 
+  - rewrite H. easy.
+Qed.
+
+Lemma multi_clear_not_adjacent : forall (gmm : graph_multi_map) from to,
+  ~ is_adjancent (<(from,to)> ~~ gmm) from to.
+Proof.
+  intros.
+  unfold is_adjancent.
+  rewrite <- multi_clear_0.
+  unfold not; intros.
+  inversion H.
+Qed.
+
+
+Definition multi_to_list_sub_list (t : (nat * partial_map nat)) :=
+  match t with
+  (x, y) => (x, List.filter (fun tpl => match tpl with
+                                       | (_, n) => negb (n =? 0)
+                                       end)
+                                       (to_list y))
+  end.
+
+Definition multi_list_flatten (t : (nat * list (nat * nat))) :=
+  match t with
+  | (n, l) => List.map (fun el => match el with
+                                  | (m, k) => (n, m, k)
+                                  end) l
+  end.
+
+Definition multi_to_list (gmm : graph_multi_map) := 
+  concat (List.map multi_list_flatten (List.map multi_to_list_sub_list (to_list gmm))).
+
+Lemma is_adjancent_in_list : forall gmm from to,
+  is_adjancent gmm from to -> exists c, In ((from, to), c) (multi_to_list gmm).
+Proof.
+  intros.
+  unfold multi_to_list.
 
 (*
 Lemma Lookup_None_iff_
